mpeg2_spec.v
@@ -1,9 +1,11 @@
 Require Import Coq.Lists.List.
 Require Import Coq.Init.Datatypes.
-Require Import Coq.Arith.Arith.
+Require Import Coq.ZArith.ZArith.
 Import ListNotations.
 
-Definition START_CODE_PREFIX := [0; 0; 1].
+Open Scope Z_scope.
+
+Definition START_CODE_PREFIX := [0%Z; 0%Z; 1%Z].
 
 Inductive start_code : Type :=
   | PACK_HEADER_CODE     : start_code
@@ -16,7 +18,7 @@ Inductive start_code : Type :=
   | PICTURE_START_CODE   : start_code
   | SEQUENCE_END_CODE    : start_code.
 
-Definition start_code_to_byte (sc : start_code) : nat :=
+Definition start_code_to_byte (sc : start_code) : Z :=
   match sc with
   | PACK_HEADER_CODE     => 186 (* 0xBA *)
   | SYSTEM_HEADER_CODE   => 187 (* 0xBB *)
@@ -29,45 +31,53 @@ Definition start_code_to_byte (sc : start_code) : nat :=
   | SEQUENCE_END_CODE    => 183 (* 0xB7 *)
   end.
 
+(* Convert Z to bits (total function) *)
+Fixpoint z_to_bits (count : nat) (val : Z) : list bool :=
+  match count with
+  | O => []
+  | S c => (z_to_bits c (val / 2)) ++ [if (val mod 2) =? 1 then true else false]
+  end.
+
+(* Group bits into Z bytes *)
+Fixpoint bits_to_z (l : list bool) : list Z :=
+  match l with
+  | b1::b2::b3::b4::b5::b6::b7::b8::rs =>
+      let val := (if b1 then 128 else 0) + (if b2 then 64 else 0) + (if b3 then 32 else 0) +
+                 (if b4 then 16 else 0) + (if b5 then 8 else 0) + (if b6 then 4 else 0) +
+                 (if b7 then 2 else 0) + (if b8 then 1 else 0) in
+      val%Z :: bits_to_z rs
+  | _ => []
+  end.
+
 Record sequence_header := {
-  horizontal_size : nat;
-  vertical_size   : nat;
-  aspect_ratio    : nat;
-  frame_rate      : nat;
-  bit_rate        : nat;
-  vbv_buffer_size : nat;
+  horizontal_size : Z;
+  vertical_size   : Z;
+  aspect_ratio    : Z;
+  frame_rate      : Z;
+  bit_rate        : Z;
+  vbv_buffer_size : Z;
 }.
 
-Definition encode_gop_header : list nat :=
-  START_CODE_PREFIX ++ [start_code_to_byte GOP_HEADER_CODE] ++
-  [0; 8; 0; 0].
-
-Definition encode_pic_header (temp_ref : nat) : list nat :=
-  START_CODE_PREFIX ++ [start_code_to_byte PICTURE_START_CODE] ++
-  [(temp_ref / 4); ((temp_ref mod 4) * 64 + 8); 255; 248].
-
-Definition encode_sequence_header (s : sequence_header) : list nat :=
+Definition encode_sequence_header (s : sequence_header) : list Z :=
   let w := s.(horizontal_size) in
   let h := s.(vertical_size) in
-  let ar := s.(aspect_ratio) in
-  let fr := s.(frame_rate) in
-  let br := s.(bit_rate) / 400 in 
-  let vbv := s.(vbv_buffer_size) / 16384 in 
+  let br := s.(bit_rate) / 400 in
+  let vbv := s.(vbv_buffer_size) / 16384 in
   START_CODE_PREFIX ++ [start_code_to_byte SEQUENCE_HEADER_CODE] ++ [
     (w / 16);
     ((w mod 16) * 16 + (h / 256));
     (h mod 256);
-    (ar * 16 + fr);
+    (s.(aspect_ratio) * 16 + s.(frame_rate));
     (br / 1024);
     ((br mod 1024) / 4);
     ((br mod 4) * 64 + 32 + (vbv / 32));
-    ((vbv mod 32) * 8 + 0)
+    ((vbv mod 32) * 8)
   ].
 
-Definition encode_pes_header (sid : nat) (len : nat) (pts : nat) : list nat :=
+Definition encode_pes_header (sid : Z) (len : Z) (pts : Z) : list Z :=
   START_CODE_PREFIX ++ [sid] ++
   [(len + 8) / 256; (len + 8) mod 256] ++
-  [128; 128; 5] ++ 
+  [128; 128; 5] ++
   [33 + (pts / 1073741824) * 2;
    (pts / 4194304) mod 256;
    (pts / 16384) mod 128 * 2 + 1;
@@ -75,17 +85,20 @@ Definition encode_pes_header (sid : nat) (len : nat) (pts : nat) : list nat :=
    (pts mod 64) * 2 + 1].
 
 Record lpcm_header := {
-  lpcm_substream_id : nat;
-  lpcm_frames : nat;
-  lpcm_ptr : nat;
-  lpcm_sample_rate : nat;
-  lpcm_bits : nat;
-  lpcm_channels : nat;
+  lpcm_subid : Z;
+  lpcm_frames : Z;
+  lpcm_ptr : Z;
+  lpcm_sample_rate : Z; (* 0=48k, 1=96k, 2=44.1k, 3=32k *)
+  lpcm_bits : Z;        (* 0=16b, 1=20b, 2=24b *)
+  lpcm_channels : Z;    (* 0=mono, 1=stereo *)
 }.
 
-Definition encode_lpcm_header (l : lpcm_header) : list nat :=
-  [ l.(lpcm_substream_id);
+Definition encode_lpcm_header (l : lpcm_header) : list Z :=
+  [ l.(lpcm_subid);
     l.(lpcm_frames);
     (l.(lpcm_ptr) / 256); (l.(lpcm_ptr) mod 256);
     (l.(lpcm_bits) * 64 + l.(lpcm_sample_rate) * 16 + l.(lpcm_channels))
   ].
+
+Theorem seq_len_z : forall s, length (encode_sequence_header s) = 12%nat.
+Proof. intros. reflexivity. Qed.
